moved each method to a separate file

lawyer/nonblocking/examples/queue/dequeue.v
@@ -8,12 +8,42 @@ From lawyer.obligations Require Import obligations_model obligations_resources o
 From lawyer Require Import sub_action_em program_logic.
 From iris.algebra Require Import auth gmap gset excl excl_auth csum mono_nat.
 From iris.base_logic.lib Require Import invariants.
-From lawyer.nonblocking.examples.queue Require Import simple_queue_utils simple_queue.
+From lawyer.nonblocking.examples.queue Require Import simple_queue_utils simple_queue right_lib.
 From heap_lang Require Import heap_lang_defs lang notation.
 
 
 Close Scope Z.
 
+
+Definition free_el: val :=
+  λ: "nd",
+    Free ("nd" +ₗ #0) ;;
+    Free ("nd" +ₗ #1)
+. 
+
+Definition get_to_free '(SQ _ _ BR FL _): val :=
+  λ: "ph",
+    if: ("ph" = !#BR)
+    then
+      let: "old_fl" := !#FL in
+      #FL <- "ph" ;;
+      "old_fl"
+    else "ph"
+.
+
+Definition dequeue '(SQ H T BR FL OHV as sq): val :=
+  λ: "q",
+    let: "c" := !#H in
+    if: ("c" = !#T)
+    then NONE
+    else
+      let: "v" := get_val "c" in
+      #OHV <- "v" ;;
+      #H <- (get_next "c") ;;
+      let: "to_free" := get_to_free sq "c" in
+      free_el "to_free" ;;
+      (SOME "v")
+.
 
 Section Dequeue.
 
@@ -28,45 +58,8 @@ Section Dequeue.
 
   Context (d: Degree).
 
-  Definition get_loc_fuel := 5.
-
   Let hGS: heap1GS Σ := iem_phys _ EM.
   Existing Instance hGS.
-
-  Lemma get_head_val_spec Q τ π q h nd fl ph od:
-    {{{ queue_inv Q ∗ ith_node h (ph, nd) ∗ dequeue_resources h fl ph od ∗
-        th_phase_frag τ π q ∗ cp_mul π d get_loc_fuel }}}
-      get_val #ph @τ
-    {{{ RET (nd.1); th_phase_frag τ π q ∗ dequeue_resources h fl ph od }}}.
-  Proof using.
-    simpl. iIntros (Φ) "([#QAT #INV] & #HEADhn & DR & PH & CPS) POST".
-    rewrite /get_val.
-    destruct nd as [v nxt]. simpl.
-    pure_steps.
-    wp_bind (_ +ₗ _)%E.
-    iApply sswp_MU_wp; [done| ].
-    iApply sswp_pure_step; [done| ].
-    MU_by_burn_cp. rewrite loc_add_0. iApply wp_value.
-    iInv "INV" as "(%hq & %h_ & %t & %br & %fl_ & %rop & %od_ & %hist & inv)" "CLOS".
-    iEval (rewrite /queue_inv_inner) in "inv".
-    iDestruct "inv" as ">(HQ & AUTHS & %ORDER & QI & DANGLE & OHV & RHI & RH & DQ)".
-    iDestruct (dequeue_resources_auth_agree with "[$] [$]") as %[<- <-].
-    iDestruct "DR" as "[HEAD FL]".
-    iDestruct (hq_auth_lookup with "[$] [$]") as %HTH.
-    iAssert (⌜ t ≠ h ⌝)%I as %NEMPTY.
-    { iIntros (->). iDestruct (queue_interp_cur_empty with "[$]") as %NO.
-      specialize (NO 0). rewrite Nat.add_0_r in NO. congruence. }
-    iDestruct (access_queue with "[$] [$] [$]") as "[HNI CLOS']".
-    { red in ORDER. lia. }
-    rewrite {1}/hn_interp. iDestruct "HNI" as "[VAL NXT]".
-    iApply sswp_MU_wp; [done| ].
-    iApply (wp_load with "VAL"). iIntros "!> VAL". 
-    MU_by_burn_cp. iApply wp_value.
-    iDestruct ("CLOS'" with "[$VAL $NXT]") as "[??]".
-    iMod ("CLOS" with "[-POST PH HEAD FL]") as "_".
-    { by iFrame. }
-    iModIntro. iApply "POST". iFrame.
-  Qed.
 
   (* TODO: unify with the proof above *)
   Lemma get_head_next_spec Q τ π q h nd fl ph od:
