lawyer/nonblocking/examples/queue/enqueue.v
@@ -8,14 +8,13 @@ From lawyer.obligations Require Import obligations_model obligations_resources o
 From lawyer Require Import sub_action_em program_logic.
 From iris.algebra Require Import auth gmap gset excl excl_auth csum mono_nat.
 From iris.base_logic.lib Require Import invariants.
-From lawyer.nonblocking.examples.queue Require Import simple_queue_utils simple_queue (* dequeue *) read_head.
+From lawyer.nonblocking.examples.queue Require Import simple_queue_utils simple_queue.
 From heap_lang Require Import heap_lang_defs lang notation.
-
 
 Close Scope Z.
 
 
-Section OtherMethods.
+Section Enqueue.
 
   Context {DegO LvlO LIM_STEPS} {OP: OP_HL DegO LvlO LIM_STEPS}.
   Context `{EM: ExecutionModel heap_lang M}.
@@ -40,23 +39,6 @@ Section OtherMethods.
 
   Let hGS: heap1GS Σ := iem_phys _ EM.
   Existing Instance hGS.
-
-  Definition set_val: val := λ: "nd" "v", ("nd" +ₗ #0) <- "v".
-  Definition set_next: val := λ: "nd" "nxt", ("nd" +ₗ #1) <- "nxt".
-
-  Definition set_node: val := 
-      λ: "nd" "v" "nxt",
-        set_val "nd" "v" ;;
-        set_next "nd" "nxt"
-  .
-
-  Definition mk_dummy_node: val :=
-    λ: <>,
-      (** dummy node has concrete field values, so we have to set them *)
-      let: "nd" := AllocN (Val $ LitV $ LitInt 2) #0 in
-      set_next "nd" #(Loc 0) ;;
-      "nd"
-  .
 
   Definition enqueue '(SQ H T BR FL OHV as sq): val :=
     λ: "v",
@@ -487,129 +469,5 @@ Section OtherMethods.
     iMod ("CLOS" with "[-]") as "_"; [| done].
     iFrame. iFrame (ORDER0). iLeft. iFrame.
   Qed.
-      
 
-  Definition read_head_dequeuer_fuel := 100.
-
-  (* TODO: refactor, unify with the beginning of dequeue *)
-  (* TODO: extract get_head_val_spec, remove import of dequeue.v *)
-  Lemma read_head_dequeuer_spec l (τ: locale heap_lang) (π: Phase) (q: Qp):
-    {{{ queue_inv l ∗ dequeue_token ∗ 
-        th_phase_frag τ π q ∗ cp_mul π d read_head_dequeuer_fuel }}}
-       read_head_dequeuer #() @ τ
-    {{{ (v: val), RET v; th_phase_frag τ π q ∗ dequeue_token }}}.
-  Proof using.
-    simpl. iIntros (Φ) "([#QAT #INV] & TOK & PH & CPS) POST".
-    rewrite /read_head_dequeuer. destruct q_sq eqn:Q_SQ.
-    pure_steps.
-
-    wp_bind (! _)%E.
-    iInv "INV" as "(%hq & %h & %t & %br & %fl & %rop & %od & %hist & inv)" "CLOS".
-    iEval (rewrite /queue_inv_inner) in "inv".
-    iDestruct "inv" as ">(HQ & AUTHS & %ORDER & QI & DANGLE & OHV & RHI & RH & DQ)".
-    
-    iApply sswp_MU_wp; [done| ].
-    iDestruct (access_queue_ends with "[$] [$]") as "(%ph & %pt & HEAD & TAIL & HT & CLOS')".
-    replace Head with (simple_queue.Head q_sq) by (by rewrite Q_SQ).
-    iApply (wp_load with "HEAD"). iIntros "!> HEAD".
-    iDestruct "DQ" as "[[%ph_ DR] | TOK']".
-    2: { by iDestruct (dequeue_token_excl with "[$] [$]") as "?". }
-    iDestruct (dequeue_res_head_agree with "DR [$]") as %<-. 
-    iDestruct (dequeue_resources_dangle_agree with "DR [$]") as %->.
-    iDestruct ("CLOS'" with "[$] [$]") as "(HQ & QI)".
-    MU_by_burn_cp. iApply wp_value.
-
-    iMod ("CLOS" with "[-POST CPS PH DR]") as "_".
-    { by iFrame. }
-    iModIntro.
-
-    (* TODO: do we need to keep track of previous values at this point? *)
-    clear t br ORDER hq.
-    clear pt rop hist.
-
-    wp_bind (Rec _ _ _)%E. pure_steps.
-
-    wp_bind (! _)%E.
-    iInv "INV" as "(%hq & %h_ & %t & %br & %fl_ & %rop & %od_ & %hist & inv)" "CLOS".
-    iEval (rewrite /queue_inv_inner) in "inv".
-    iDestruct "inv" as ">(HQ & AUTHS & %ORDER & QI & DANGLE & OHV & RHI & RH & DQ)".
-    iApply sswp_MU_wp; [done| ].
-    iDestruct (access_queue_ends with "[$] [$]") as "(%ph_ & %pt & HEAD & TAIL & #HT & CLOS')".
-    replace Tail with (simple_queue.Tail q_sq) by (by rewrite Q_SQ).
-    iApply (wp_load with "[$]"). iIntros "!> TAIL".
-    iDestruct (dequeue_res_head_agree with "DR [$]") as %->. 
-    iDestruct (dequeue_resources_auth_agree with "DR [$]") as %[<- <-].
-    iDestruct (take_snapshot with "[$]") as "#SHT".
-    iDestruct "DQ" as "[(% & DR') | TOK]".
-    { by iDestruct (dequeue_resources_excl with "DR DR'") as "?". }
-
-    iDestruct ("CLOS'" with "[$] [$]") as "(HQ & QI)".
-    MU_by_burn_cp. iApply wp_value.
-    iMod ("CLOS" with "[-POST CPS PH DR]") as "_".
-    { by iFrame. }
-    iModIntro.
-
-    wp_bind (Rec _ _ _)%E. pure_steps.    
-
-    (* TODO: do we need to keep track of previous values at this point? *)
-    (* clear br hob od ohv ORDER SAFE_BR hq. *)
-    iClear "SHT". 
-    clear hist hq od_ (* ORDER *) rop (* br *).    
-
-    wp_bind (_ = _)%E.
-    iApply sswp_MU_wp; [done| ].
-    iApply sswp_pure_step.
-    { set_solver. }
-    MU_by_burn_cp. iApply wp_value.
-
-    (* destruct bool_decide. *)
-    iDestruct "HT" as "[[%GE <-] | (%NEMPTY & %ndh & #HTH)]". 
-    { assert (t = h) as ->.
-      { red in ORDER. lia. }
-      rewrite bool_decide_true; [| done]. 
-      iApply sswp_MU_wp_fupd; [done| ]. 
-      iInv "INV" as "(%hq & %h_ & %t & %br' & %fl_ & %rop & %od_ & %hist & inv)" "CLOS".
-      iEval (rewrite /queue_inv_inner) in "inv".
-      clear ORDER. 
-      iDestruct "inv" as ">(HQ & AUTHS & %ORDER & QI & DANGLE & OHV & RHI & RH & DQ)".
-      iModIntro.
-      iApply sswp_pure_step; [done| ].
-      do 2 iNext. MU_by_burn_cp.
-      iDestruct "DQ" as "[(% & DR') | TOK]".
-      { by iDestruct (dequeue_resources_excl with "[$] [$]") as "?". }
-      iDestruct (dequeue_resources_auth_agree with "[$] [$]") as %[-> ->]. 
-      iMod ("CLOS" with "[-POST CPS PH TOK]") as "_".
-      { by iFrame. }
-      iModIntro. pure_steps.
-      iApply "POST". iFrame. }
-
-    rewrite bool_decide_false; [| set_solver]. pure_steps.
-    split_cps "CPS" get_loc_fuel; [cbv; lia| ].
-
-    (* TODO: move *)
-    From lawyer.nonblocking.examples.queue Require Import dequeue.
-  
-    iApply (get_head_val_spec with "[-POST CPS]").
-    { iFrame "#∗". }
-    iIntros "!> [PH DR]".
-
-    iApply sswp_MU_wp_fupd; [done| ]. 
-    iInv "INV" as "(%hq & %h_ & %t' & %br' & %fl_ & %rop & %od & %hist & inv)" "CLOS".
-    iEval (rewrite /queue_inv_inner) in "inv".
-    iDestruct "inv" as ">(HQ & AUTHS & %ORDER' & QI & DANGLE & OHV & RHI & RH & DQ)".
-    iDestruct "DQ" as "[(% & DR') | TOK]".
-    { by iDestruct (dequeue_resources_excl with "DR DR'") as "?". }
-    (* iDestruct (dequeue_res_head_agree with "DR [$]") as %->.  *)
-    iDestruct (dequeue_resources_auth_agree with "DR [$]") as %[<- <-].
-    iDestruct (dequeue_resources_dangle_agree with "DR [$]") as %->.
-
-    iModIntro. iApply sswp_pure_step; [done| ]. 
-    MU_by_burn_cp. simpl.
-    iMod ("CLOS" with "[-POST CPS PH TOK]") as "_".
-    { by iFrame. }
- 
-    iModIntro. pure_steps.
-    iApply "POST". iFrame.
-  Qed.    
-
-End OtherMethods.
+End Enqueue.
