lawyer/nonblocking/examples/queue/read_head_dequeuer.v
@@ -1,0 +1,160 @@
+From iris.base_logic Require Export gen_heap.
+From iris.proofmode Require Import tactics coq_tactics.
+From iris.bi.lib Require Import fixpoint.
+From trillium.program_logic Require Export weakestpre adequacy ectx_lifting.
+From fairness Require Import utils.
+From lawyer.examples Require Import obls_tactics.
+From lawyer.obligations Require Import obligations_model obligations_resources obligations_am obligations_em obligations_logic env_helpers.
+From lawyer Require Import sub_action_em program_logic.
+From iris.algebra Require Import auth gmap gset excl excl_auth csum mono_nat.
+From iris.base_logic.lib Require Import invariants.
+From lawyer.nonblocking.examples.queue Require Import simple_queue_utils simple_queue right_lib.
+From heap_lang Require Import heap_lang_defs lang notation.
+
+
+Close Scope Z.
+
+
+Section ReadHeadDequeuer.      
+
+  Context {DegO LvlO LIM_STEPS} {OP: OP_HL DegO LvlO LIM_STEPS}.
+  Context `{EM: ExecutionModel heap_lang M}.
+  Notation "'Degree'" := (om_hl_Degree). 
+  Notation "'Level'" := (om_hl_Level).  
+
+  Context {Σ} {OHE: OM_HL_Env OP EM Σ}.
+  Context {QL: QueueG Σ}.
+
+  Definition read_head_dequeuer: val := 
+    λ: <>,
+      let: "ch" := !#(Head q_sq) in
+      let: "ct" := !#(Tail q_sq) in
+      if: "ch" = "ct" then NONE
+      else SOME (get_val "ch")
+  .
+
+  Context (d: Degree).
+
+  Let hGS: heap1GS Σ := iem_phys _ EM.
+  Existing Instance hGS.
+  Definition read_head_dequeuer_fuel := 100.
+
+  (* TODO: refactor, unify with the beginning of dequeue *)
+  (* TODO: extract get_head_val_spec, remove import of dequeue.v *)
+  Lemma read_head_dequeuer_spec l (τ: locale heap_lang) (π: Phase) (q: Qp):
+    {{{ queue_inv l ∗ dequeue_token ∗ 
+        th_phase_frag τ π q ∗ cp_mul π d read_head_dequeuer_fuel }}}
+       read_head_dequeuer #() @ τ
+    {{{ (v: val), RET v; th_phase_frag τ π q ∗ dequeue_token }}}.
+  Proof using.
+    simpl. iIntros (Φ) "([#QAT #INV] & TOK & PH & CPS) POST".
+    rewrite /read_head_dequeuer. destruct q_sq eqn:Q_SQ.
+    pure_steps.
+
+    wp_bind (! _)%E.
+    iInv "INV" as "(%hq & %h & %t & %br & %fl & %rop & %od & %hist & inv)" "CLOS".
+    iEval (rewrite /queue_inv_inner) in "inv".
+    iDestruct "inv" as ">(HQ & AUTHS & %ORDER & QI & DANGLE & OHV & RHI & RH & DQ)".
+    
+    iApply sswp_MU_wp; [done| ].
+    iDestruct (access_queue_ends with "[$] [$]") as "(%ph & %pt & HEAD & TAIL & HT & CLOS')".
+    replace Head with (simple_queue.Head q_sq) by (by rewrite Q_SQ).
+    iApply (wp_load with "HEAD"). iIntros "!> HEAD".
+    iDestruct "DQ" as "[[%ph_ DR] | TOK']".
+    2: { by iDestruct (dequeue_token_excl with "[$] [$]") as "?". }
+    iDestruct (dequeue_res_head_agree with "DR [$]") as %<-. 
+    iDestruct (dequeue_resources_dangle_agree with "DR [$]") as %->.
+    iDestruct ("CLOS'" with "[$] [$]") as "(HQ & QI)".
+    MU_by_burn_cp. iApply wp_value.
+
+    iMod ("CLOS" with "[-POST CPS PH DR]") as "_".
+    { by iFrame. }
+    iModIntro.
+
+    (* TODO: do we need to keep track of previous values at this point? *)
+    clear t br ORDER hq.
+    clear pt rop hist.
+
+    wp_bind (Rec _ _ _)%E. pure_steps.
+
+    wp_bind (! _)%E.
+    iInv "INV" as "(%hq & %h_ & %t & %br & %fl_ & %rop & %od_ & %hist & inv)" "CLOS".
+    iEval (rewrite /queue_inv_inner) in "inv".
+    iDestruct "inv" as ">(HQ & AUTHS & %ORDER & QI & DANGLE & OHV & RHI & RH & DQ)".
+    iApply sswp_MU_wp; [done| ].
+    iDestruct (access_queue_ends with "[$] [$]") as "(%ph_ & %pt & HEAD & TAIL & #HT & CLOS')".
+    replace Tail with (simple_queue.Tail q_sq) by (by rewrite Q_SQ).
+    iApply (wp_load with "[$]"). iIntros "!> TAIL".
+    iDestruct (dequeue_res_head_agree with "DR [$]") as %->. 
+    iDestruct (dequeue_resources_auth_agree with "DR [$]") as %[<- <-].
+    iDestruct (take_snapshot with "[$]") as "#SHT".
+    iDestruct "DQ" as "[(% & DR') | TOK]".
+    { by iDestruct (dequeue_resources_excl with "DR DR'") as "?". }
+
+    iDestruct ("CLOS'" with "[$] [$]") as "(HQ & QI)".
+    MU_by_burn_cp. iApply wp_value.
+    iMod ("CLOS" with "[-POST CPS PH DR]") as "_".
+    { by iFrame. }
+    iModIntro.
+
+    wp_bind (Rec _ _ _)%E. pure_steps.    
+
+    (* TODO: do we need to keep track of previous values at this point? *)
+    (* clear br hob od ohv ORDER SAFE_BR hq. *)
+    iClear "SHT". 
+    clear hist hq od_ (* ORDER *) rop (* br *).    
+
+    wp_bind (_ = _)%E.
+    iApply sswp_MU_wp; [done| ].
+    iApply sswp_pure_step.
+    { set_solver. }
+    MU_by_burn_cp. iApply wp_value.
+
+    (* destruct bool_decide. *)
+    iDestruct "HT" as "[[%GE <-] | (%NEMPTY & %ndh & #HTH)]". 
+    { assert (t = h) as ->.
+      { red in ORDER. lia. }
+      rewrite bool_decide_true; [| done]. 
+      iApply sswp_MU_wp_fupd; [done| ]. 
+      iInv "INV" as "(%hq & %h_ & %t & %br' & %fl_ & %rop & %od_ & %hist & inv)" "CLOS".
+      iEval (rewrite /queue_inv_inner) in "inv".
+      clear ORDER. 
+      iDestruct "inv" as ">(HQ & AUTHS & %ORDER & QI & DANGLE & OHV & RHI & RH & DQ)".
+      iModIntro.
+      iApply sswp_pure_step; [done| ].
+      do 2 iNext. MU_by_burn_cp.
+      iDestruct "DQ" as "[(% & DR') | TOK]".
+      { by iDestruct (dequeue_resources_excl with "[$] [$]") as "?". }
+      iDestruct (dequeue_resources_auth_agree with "[$] [$]") as %[-> ->]. 
+      iMod ("CLOS" with "[-POST CPS PH TOK]") as "_".
+      { by iFrame. }
+      iModIntro. pure_steps.
+      iApply "POST". iFrame. }
+
+    rewrite bool_decide_false; [| set_solver]. pure_steps.
+    split_cps "CPS" get_loc_fuel; [cbv; lia| ].
+  
+    iApply (get_head_val_spec with "[-POST CPS]").
+    { iFrame "#∗". }
+    iIntros "!> [PH DR]".
+
+    iApply sswp_MU_wp_fupd; [done| ]. 
+    iInv "INV" as "(%hq & %h_ & %t' & %br' & %fl_ & %rop & %od & %hist & inv)" "CLOS".
+    iEval (rewrite /queue_inv_inner) in "inv".
+    iDestruct "inv" as ">(HQ & AUTHS & %ORDER' & QI & DANGLE & OHV & RHI & RH & DQ)".
+    iDestruct "DQ" as "[(% & DR') | TOK]".
+    { by iDestruct (dequeue_resources_excl with "DR DR'") as "?". }
+    (* iDestruct (dequeue_res_head_agree with "DR [$]") as %->.  *)
+    iDestruct (dequeue_resources_auth_agree with "DR [$]") as %[<- <-].
+    iDestruct (dequeue_resources_dangle_agree with "DR [$]") as %->.
+
+    iModIntro. iApply sswp_pure_step; [done| ]. 
+    MU_by_burn_cp. simpl.
+    iMod ("CLOS" with "[-POST CPS PH TOK]") as "_".
+    { by iFrame. }
+ 
+    iModIntro. pure_steps.
+    iApply "POST". iFrame.
+  Qed.    
+
+End ReadHeadDequeuer.
