lawyer/nonblocking/examples/queue/right_lib.v
@@ -1,0 +1,69 @@
+From iris.base_logic Require Export gen_heap.
+From iris.proofmode Require Import tactics coq_tactics.
+From iris.bi.lib Require Import fixpoint.
+From trillium.program_logic Require Export weakestpre adequacy ectx_lifting.
+From fairness Require Import utils.
+From lawyer.examples Require Import obls_tactics.
+From lawyer.obligations Require Import obligations_model obligations_resources obligations_am obligations_em obligations_logic env_helpers.
+From lawyer Require Import sub_action_em program_logic.
+From iris.algebra Require Import auth gmap gset excl excl_auth csum mono_nat.
+From iris.base_logic.lib Require Import invariants.
+From lawyer.nonblocking.examples.queue Require Import simple_queue_utils simple_queue.
+From heap_lang Require Import heap_lang_defs lang notation.
+
+Close Scope Z.
+
+Section RightUtils.
+
+  Context {DegO LvlO LIM_STEPS} {OP: OP_HL DegO LvlO LIM_STEPS}.
+  Context `{EM: ExecutionModel heap_lang M}.
+  Notation "'Degree'" := (om_hl_Degree). 
+  Notation "'Level'" := (om_hl_Level).  
+
+  Context {Σ} {OHE: OM_HL_Env OP EM Σ}.
+  (* Existing Instance OHE.  *)
+  Context {QL: QueueG Σ}.
+
+  Context (d: Degree).
+
+  Definition get_loc_fuel := 5.
+
+  Let hGS: heap1GS Σ := iem_phys _ EM.
+  Existing Instance hGS.
+
+  Lemma get_head_val_spec Q τ π q h nd fl ph od:
+    {{{ queue_inv Q ∗ ith_node h (ph, nd) ∗ dequeue_resources h fl ph od ∗
+        th_phase_frag τ π q ∗ cp_mul π d get_loc_fuel }}}
+      get_val #ph @τ
+    {{{ RET (nd.1); th_phase_frag τ π q ∗ dequeue_resources h fl ph od }}}.
+  Proof using.
+    simpl. iIntros (Φ) "([#QAT #INV] & #HEADhn & DR & PH & CPS) POST".
+    rewrite /get_val.
+    destruct nd as [v nxt]. simpl.
+    pure_steps.
+    wp_bind (_ +ₗ _)%E.
+    iApply sswp_MU_wp; [done| ].
+    iApply sswp_pure_step; [done| ].
+    MU_by_burn_cp. rewrite loc_add_0. iApply wp_value.
+    iInv "INV" as "(%hq & %h_ & %t & %br & %fl_ & %rop & %od_ & %hist & inv)" "CLOS".
+    iEval (rewrite /queue_inv_inner) in "inv".
+    iDestruct "inv" as ">(HQ & AUTHS & %ORDER & QI & DANGLE & OHV & RHI & RH & DQ)".
+    iDestruct (dequeue_resources_auth_agree with "[$] [$]") as %[<- <-].
+    iDestruct "DR" as "[HEAD FL]".
+    iDestruct (hq_auth_lookup with "[$] [$]") as %HTH.
+    iAssert (⌜ t ≠ h ⌝)%I as %NEMPTY.
+    { iIntros (->). iDestruct (queue_interp_cur_empty with "[$]") as %NO.
+      specialize (NO 0). rewrite Nat.add_0_r in NO. congruence. }
+    iDestruct (access_queue with "[$] [$] [$]") as "[HNI CLOS']".
+    { red in ORDER. lia. }
+    rewrite {1}/hn_interp. iDestruct "HNI" as "[VAL NXT]".
+    iApply sswp_MU_wp; [done| ].
+    iApply (wp_load with "VAL"). iIntros "!> VAL". 
+    MU_by_burn_cp. iApply wp_value.
+    iDestruct ("CLOS'" with "[$VAL $NXT]") as "[??]".
+    iMod ("CLOS" with "[-POST PH HEAD FL]") as "_".
+    { by iFrame. }
+    iModIntro. iApply "POST". iFrame.
+  Qed.
+
+End RightUtils.
